fixed spec - size as param

_build/default/src/proofs/solswitch/generated_proof_SML_trySwitch.v.d
@@ -1,0 +1,2 @@
+generated_proof_SML_trySwitch.vo generated_proof_SML_trySwitch.glob generated_proof_SML_trySwitch.v.beautified generated_proof_SML_trySwitch.required_vo: generated_proof_SML_trySwitch.v ./generated_code.vo ./generated_spec.vo
+generated_proof_SML_trySwitch.vio: generated_proof_SML_trySwitch.v ./generated_code.vio ./generated_spec.vio
