src/proofs/solswitch/generated_code.v
@@ -6,67 +6,74 @@ Set Default Proof Using "Type".
 (* Generated from [src/solswitch.c]. *)
 Section code.
   Definition file_0 : string := "src/solswitch.c".
-  Definition loc_2 : location_info := LocationInfo file_0 31 53 31 62.
-  Definition loc_3 : location_info := LocationInfo file_0 31 60 31 61.
-  Definition loc_6 : location_info := LocationInfo file_0 41 1 44 2.
-  Definition loc_7 : location_info := LocationInfo file_0 41 23 44 2.
-  Definition loc_8 : location_info := LocationInfo file_0 43 2 43 17.
-  Definition loc_9 : location_info := LocationInfo file_0 43 2 43 12.
-  Definition loc_10 : location_info := LocationInfo file_0 43 2 43 5.
-  Definition loc_11 : location_info := LocationInfo file_0 43 2 43 5.
-  Definition loc_12 : location_info := LocationInfo file_0 43 15 43 16.
-  Definition loc_13 : location_info := LocationInfo file_0 41 1 44 2.
-  Definition loc_14 : location_info := LocationInfo file_0 41 6 41 21.
-  Definition loc_15 : location_info := LocationInfo file_0 41 6 41 7.
-  Definition loc_16 : location_info := LocationInfo file_0 41 11 41 21.
-  Definition loc_17 : location_info := LocationInfo file_0 41 11 41 21.
-  Definition loc_18 : location_info := LocationInfo file_0 41 11 41 14.
-  Definition loc_19 : location_info := LocationInfo file_0 41 11 41 14.
-  Definition loc_22 : location_info := LocationInfo file_0 65 4 65 58.
-  Definition loc_23 : location_info := LocationInfo file_0 66 4 72 5.
-  Definition loc_24 : location_info := LocationInfo file_0 66 22 72 5.
-  Definition loc_25 : location_info := LocationInfo file_0 67 8 71 9.
-  Definition loc_26 : location_info := LocationInfo file_0 67 26 71 9.
-  Definition loc_27 : location_info := LocationInfo file_0 68 12 70 13.
-  Definition loc_28 : location_info := LocationInfo file_0 68 63 70 13.
-  Definition loc_29 : location_info := LocationInfo file_0 69 15 69 42.
-  Definition loc_30 : location_info := LocationInfo file_0 69 15 69 36.
-  Definition loc_31 : location_info := LocationInfo file_0 69 15 69 36.
-  Definition loc_32 : location_info := LocationInfo file_0 69 37 69 40.
-  Definition loc_33 : location_info := LocationInfo file_0 69 37 69 40.
-  Definition loc_34 : location_info := LocationInfo file_0 68 12 70 13.
-  Definition loc_35 : location_info := LocationInfo file_0 68 15 68 62.
-  Definition loc_36 : location_info := LocationInfo file_0 68 15 68 36.
-  Definition loc_37 : location_info := LocationInfo file_0 68 15 68 31.
-  Definition loc_38 : location_info := LocationInfo file_0 68 15 68 31.
-  Definition loc_39 : location_info := LocationInfo file_0 68 15 68 27.
-  Definition loc_40 : location_info := LocationInfo file_0 68 15 68 18.
-  Definition loc_41 : location_info := LocationInfo file_0 68 15 68 18.
-  Definition loc_42 : location_info := LocationInfo file_0 68 35 68 36.
-  Definition loc_43 : location_info := LocationInfo file_0 68 40 68 62.
-  Definition loc_44 : location_info := LocationInfo file_0 68 40 68 56.
-  Definition loc_45 : location_info := LocationInfo file_0 68 40 68 56.
-  Definition loc_46 : location_info := LocationInfo file_0 68 40 68 52.
-  Definition loc_47 : location_info := LocationInfo file_0 68 40 68 43.
-  Definition loc_48 : location_info := LocationInfo file_0 68 40 68 43.
-  Definition loc_49 : location_info := LocationInfo file_0 68 60 68 62.
-  Definition loc_50 : location_info := LocationInfo file_0 67 8 71 9.
-  Definition loc_51 : location_info := LocationInfo file_0 67 11 67 25.
-  Definition loc_52 : location_info := LocationInfo file_0 67 11 67 20.
-  Definition loc_53 : location_info := LocationInfo file_0 67 11 67 20.
-  Definition loc_54 : location_info := LocationInfo file_0 67 24 67 25.
-  Definition loc_55 : location_info := LocationInfo file_0 66 4 72 5.
-  Definition loc_56 : location_info := LocationInfo file_0 66 7 66 21.
-  Definition loc_57 : location_info := LocationInfo file_0 66 7 66 16.
-  Definition loc_58 : location_info := LocationInfo file_0 66 7 66 16.
-  Definition loc_59 : location_info := LocationInfo file_0 66 20 66 21.
-  Definition loc_60 : location_info := LocationInfo file_0 65 24 65 57.
-  Definition loc_61 : location_info := LocationInfo file_0 65 24 65 42.
-  Definition loc_62 : location_info := LocationInfo file_0 65 24 65 42.
-  Definition loc_63 : location_info := LocationInfo file_0 65 43 65 56.
-  Definition loc_64 : location_info := LocationInfo file_0 65 44 65 56.
-  Definition loc_65 : location_info := LocationInfo file_0 65 44 65 47.
-  Definition loc_66 : location_info := LocationInfo file_0 65 44 65 47.
+  Definition loc_2 : location_info := LocationInfo file_0 29 53 29 62.
+  Definition loc_3 : location_info := LocationInfo file_0 29 60 29 61.
+  Definition loc_6 : location_info := LocationInfo file_0 39 1 42 2.
+  Definition loc_7 : location_info := LocationInfo file_0 39 23 42 2.
+  Definition loc_8 : location_info := LocationInfo file_0 41 2 41 17.
+  Definition loc_9 : location_info := LocationInfo file_0 41 2 41 12.
+  Definition loc_10 : location_info := LocationInfo file_0 41 2 41 5.
+  Definition loc_11 : location_info := LocationInfo file_0 41 2 41 5.
+  Definition loc_12 : location_info := LocationInfo file_0 41 15 41 16.
+  Definition loc_13 : location_info := LocationInfo file_0 39 1 42 2.
+  Definition loc_14 : location_info := LocationInfo file_0 39 6 39 21.
+  Definition loc_15 : location_info := LocationInfo file_0 39 6 39 7.
+  Definition loc_16 : location_info := LocationInfo file_0 39 11 39 21.
+  Definition loc_17 : location_info := LocationInfo file_0 39 11 39 21.
+  Definition loc_18 : location_info := LocationInfo file_0 39 11 39 14.
+  Definition loc_19 : location_info := LocationInfo file_0 39 11 39 14.
+  Definition loc_22 : location_info := LocationInfo file_0 59 4 65 5.
+  Definition loc_23 : location_info := LocationInfo file_0 59 19 65 5.
+  Definition loc_24 : location_info := LocationInfo file_0 60 8 64 9.
+  Definition loc_25 : location_info := LocationInfo file_0 60 23 64 9.
+  Definition loc_26 : location_info := LocationInfo file_0 61 12 63 13.
+  Definition loc_27 : location_info := LocationInfo file_0 61 63 63 13.
+  Definition loc_28 : location_info := LocationInfo file_0 62 15 62 42.
+  Definition loc_29 : location_info := LocationInfo file_0 62 15 62 36.
+  Definition loc_30 : location_info := LocationInfo file_0 62 15 62 36.
+  Definition loc_31 : location_info := LocationInfo file_0 62 37 62 40.
+  Definition loc_32 : location_info := LocationInfo file_0 62 37 62 40.
+  Definition loc_33 : location_info := LocationInfo file_0 61 12 63 13.
+  Definition loc_34 : location_info := LocationInfo file_0 61 15 61 62.
+  Definition loc_35 : location_info := LocationInfo file_0 61 15 61 36.
+  Definition loc_36 : location_info := LocationInfo file_0 61 15 61 31.
+  Definition loc_37 : location_info := LocationInfo file_0 61 15 61 31.
+  Definition loc_38 : location_info := LocationInfo file_0 61 15 61 27.
+  Definition loc_39 : location_info := LocationInfo file_0 61 15 61 18.
+  Definition loc_40 : location_info := LocationInfo file_0 61 15 61 18.
+  Definition loc_41 : location_info := LocationInfo file_0 61 35 61 36.
+  Definition loc_42 : location_info := LocationInfo file_0 61 40 61 62.
+  Definition loc_43 : location_info := LocationInfo file_0 61 40 61 56.
+  Definition loc_44 : location_info := LocationInfo file_0 61 40 61 56.
+  Definition loc_45 : location_info := LocationInfo file_0 61 40 61 52.
+  Definition loc_46 : location_info := LocationInfo file_0 61 40 61 43.
+  Definition loc_47 : location_info := LocationInfo file_0 61 40 61 43.
+  Definition loc_48 : location_info := LocationInfo file_0 61 60 61 62.
+  Definition loc_49 : location_info := LocationInfo file_0 60 8 64 9.
+  Definition loc_50 : location_info := LocationInfo file_0 60 11 60 22.
+  Definition loc_51 : location_info := LocationInfo file_0 60 11 60 17.
+  Definition loc_52 : location_info := LocationInfo file_0 60 11 60 17.
+  Definition loc_53 : location_info := LocationInfo file_0 60 21 60 22.
+  Definition loc_54 : location_info := LocationInfo file_0 59 4 65 5.
+  Definition loc_55 : location_info := LocationInfo file_0 59 7 59 18.
+  Definition loc_56 : location_info := LocationInfo file_0 59 7 59 13.
+  Definition loc_57 : location_info := LocationInfo file_0 59 7 59 13.
+  Definition loc_58 : location_info := LocationInfo file_0 59 17 59 18.
+  Definition loc_61 : location_info := LocationInfo file_0 78 4 78 58.
+  Definition loc_62 : location_info := LocationInfo file_0 79 4 79 34.
+  Definition loc_63 : location_info := LocationInfo file_0 79 4 79 17.
+  Definition loc_64 : location_info := LocationInfo file_0 79 4 79 17.
+  Definition loc_65 : location_info := LocationInfo file_0 79 18 79 21.
+  Definition loc_66 : location_info := LocationInfo file_0 79 18 79 21.
+  Definition loc_67 : location_info := LocationInfo file_0 79 23 79 32.
+  Definition loc_68 : location_info := LocationInfo file_0 79 23 79 32.
+  Definition loc_69 : location_info := LocationInfo file_0 78 24 78 57.
+  Definition loc_70 : location_info := LocationInfo file_0 78 24 78 42.
+  Definition loc_71 : location_info := LocationInfo file_0 78 24 78 42.
+  Definition loc_72 : location_info := LocationInfo file_0 78 43 78 56.
+  Definition loc_73 : location_info := LocationInfo file_0 78 44 78 56.
+  Definition loc_74 : location_info := LocationInfo file_0 78 44 78 47.
+  Definition loc_75 : location_info := LocationInfo file_0 78 44 78 47.
 
   (* Definition of struct [div]. *)
   Program Definition struct_div := {|
@@ -159,8 +166,62 @@ Section code.
     )%E
   |}.
 
+  (* Definition of function [SML_trySwitch]. *)
+  Definition impl_SML_trySwitch (global_SML_switchTheSolenoid : loc): function := {|
+    f_args := [
+      ("ssp", void*);
+      ("length", it_layout u8)
+    ];
+    f_local_vars := [
+    ];
+    f_init := "#0";
+    f_code := (
+      <[ "#0" :=
+        locinfo: loc_55 ;
+        if{IntOp i32}: LocInfoE loc_55 ((LocInfoE loc_56 (UnOp (CastOp $ IntOp i32) (IntOp u8) (LocInfoE loc_56 (use{IntOp u8} (LocInfoE loc_57 ("length")))))) !={IntOp i32, IntOp i32, i32} (LocInfoE loc_58 (i2v 0 i32)))
+        then
+        locinfo: loc_50 ;
+          Goto "#1"
+        else
+        Goto "#6"
+      ]> $
+      <[ "#1" :=
+        locinfo: loc_50 ;
+        if{IntOp i32}: LocInfoE loc_50 ((LocInfoE loc_51 (UnOp (CastOp $ IntOp i32) (IntOp u8) (LocInfoE loc_51 (use{IntOp u8} (LocInfoE loc_52 ("length")))))) ={IntOp i32, IntOp i32, i32} (LocInfoE loc_53 (i2v 8 i32)))
+        then
+        locinfo: loc_34 ;
+          Goto "#2"
+        else
+        Goto "#5"
+      ]> $
+      <[ "#2" :=
+        locinfo: loc_34 ;
+        if{IntOp i32}: LocInfoE loc_34 ((LocInfoE loc_35 ((LocInfoE loc_36 (UnOp (CastOp $ IntOp i32) (IntOp u8) (LocInfoE loc_36 (use{IntOp u8} (LocInfoE loc_37 ((LocInfoE loc_38 ((LocInfoE loc_39 (!{PtrOp} (LocInfoE loc_40 ("ssp")))) at{struct_SolenoidSwitchingParams_t} "handler")) at{struct_ComHandler_t} "msg")))))) ={IntOp i32, IntOp i32, i32} (LocInfoE loc_41 (i2v 7 i32)))) ||{IntOp i32, IntOp i32, i32} (LocInfoE loc_42 ((LocInfoE loc_43 (UnOp (CastOp $ IntOp i32) (IntOp u8) (LocInfoE loc_43 (use{IntOp u8} (LocInfoE loc_44 ((LocInfoE loc_45 ((LocInfoE loc_46 (!{PtrOp} (LocInfoE loc_47 ("ssp")))) at{struct_SolenoidSwitchingParams_t} "handler")) at{struct_ComHandler_t} "msg")))))) ={IntOp i32, IntOp i32, i32} (LocInfoE loc_48 (i2v 12 i32)))))
+        then
+        locinfo: loc_28 ;
+          Goto "#3"
+        else
+        Goto "#4"
+      ]> $
+      <[ "#3" :=
+        locinfo: loc_28 ;
+        expr: (LocInfoE loc_28 (Call (LocInfoE loc_30 (global_SML_switchTheSolenoid)) [@{expr} LocInfoE loc_31 (use{PtrOp} (LocInfoE loc_32 ("ssp"))) ])) ;
+        Return (VOID)
+      ]> $
+      <[ "#4" :=
+        Return (VOID)
+      ]> $
+      <[ "#5" :=
+        Return (VOID)
+      ]> $
+      <[ "#6" :=
+        Return (VOID)
+      ]> $∅
+    )%E
+  |}.
+
   (* Definition of function [SML_handleReceivedMsgs]. *)
-  Definition impl_SML_handleReceivedMsgs (global_SCH_recieveFullMsg global_SML_switchTheSolenoid : loc): function := {|
+  Definition impl_SML_handleReceivedMsgs (global_SCH_recieveFullMsg global_SML_trySwitch : loc): function := {|
     f_args := [
       ("ssp", void*)
     ];
@@ -171,45 +232,10 @@ Section code.
     f_code := (
       <[ "#0" :=
         "rxMsgSize" <-{ IntOp u8 }
-          LocInfoE loc_60 (Call (LocInfoE loc_62 (global_SCH_recieveFullMsg)) [@{expr} LocInfoE loc_63 (&(LocInfoE loc_64 ((LocInfoE loc_65 (!{PtrOp} (LocInfoE loc_66 ("ssp")))) at{struct_SolenoidSwitchingParams_t} "handler"))) ]) ;
-        locinfo: loc_56 ;
-        if{IntOp i32}: LocInfoE loc_56 ((LocInfoE loc_57 (UnOp (CastOp $ IntOp i32) (IntOp u8) (LocInfoE loc_57 (use{IntOp u8} (LocInfoE loc_58 ("rxMsgSize")))))) !={IntOp i32, IntOp i32, i32} (LocInfoE loc_59 (i2v 0 i32)))
-        then
-        locinfo: loc_51 ;
-          Goto "#1"
-        else
-        Goto "#6"
-      ]> $
-      <[ "#1" :=
-        locinfo: loc_51 ;
-        if{IntOp i32}: LocInfoE loc_51 ((LocInfoE loc_52 (UnOp (CastOp $ IntOp i32) (IntOp u8) (LocInfoE loc_52 (use{IntOp u8} (LocInfoE loc_53 ("rxMsgSize")))))) ={IntOp i32, IntOp i32, i32} (LocInfoE loc_54 (i2v 8 i32)))
-        then
-        locinfo: loc_35 ;
-          Goto "#2"
-        else
-        Goto "#5"
-      ]> $
-      <[ "#2" :=
-        locinfo: loc_35 ;
-        if{IntOp i32}: LocInfoE loc_35 ((LocInfoE loc_36 ((LocInfoE loc_37 (UnOp (CastOp $ IntOp i32) (IntOp u8) (LocInfoE loc_37 (use{IntOp u8} (LocInfoE loc_38 ((LocInfoE loc_39 ((LocInfoE loc_40 (!{PtrOp} (LocInfoE loc_41 ("ssp")))) at{struct_SolenoidSwitchingParams_t} "handler")) at{struct_ComHandler_t} "msg")))))) ={IntOp i32, IntOp i32, i32} (LocInfoE loc_42 (i2v 7 i32)))) ||{IntOp i32, IntOp i32, i32} (LocInfoE loc_43 ((LocInfoE loc_44 (UnOp (CastOp $ IntOp i32) (IntOp u8) (LocInfoE loc_44 (use{IntOp u8} (LocInfoE loc_45 ((LocInfoE loc_46 ((LocInfoE loc_47 (!{PtrOp} (LocInfoE loc_48 ("ssp")))) at{struct_SolenoidSwitchingParams_t} "handler")) at{struct_ComHandler_t} "msg")))))) ={IntOp i32, IntOp i32, i32} (LocInfoE loc_49 (i2v 12 i32)))))
-        then
-        locinfo: loc_29 ;
-          Goto "#3"
-        else
-        Goto "#4"
-      ]> $
-      <[ "#3" :=
-        locinfo: loc_29 ;
-        expr: (LocInfoE loc_29 (Call (LocInfoE loc_31 (global_SML_switchTheSolenoid)) [@{expr} LocInfoE loc_32 (use{PtrOp} (LocInfoE loc_33 ("ssp"))) ])) ;
-        Return (VOID)
-      ]> $
-      <[ "#4" :=
-        Return (VOID)
-      ]> $
-      <[ "#5" :=
-        Return (VOID)
-      ]> $
-      <[ "#6" :=
+          LocInfoE loc_69 (Call (LocInfoE loc_71 (global_SCH_recieveFullMsg)) [@{expr} LocInfoE loc_72 (&(LocInfoE loc_73 ((LocInfoE loc_74 (!{PtrOp} (LocInfoE loc_75 ("ssp")))) at{struct_SolenoidSwitchingParams_t} "handler"))) ]) ;
+        locinfo: loc_62 ;
+        expr: (LocInfoE loc_62 (Call (LocInfoE loc_64 (global_SML_trySwitch)) [@{expr} LocInfoE loc_65 (use{PtrOp} (LocInfoE loc_66 ("ssp"))) ;
+        LocInfoE loc_67 (use{IntOp u8} (LocInfoE loc_68 ("rxMsgSize"))) ])) ;
         Return (VOID)
       ]> $∅
     )%E
