src/proofs/solswitch/generated_proof_SML_handleReceivedMsgs.v
@@ -8,10 +8,10 @@ Section proof_SML_handleReceivedMsgs.
   Context `{!typeG Σ} `{!globalG Σ}.
 
   (* Typing proof for [SML_handleReceivedMsgs]. *)
-  Lemma type_SML_handleReceivedMsgs (global_SCH_recieveFullMsg global_SML_switchTheSolenoid : loc) :
+  Lemma type_SML_handleReceivedMsgs (global_SCH_recieveFullMsg global_SML_trySwitch : loc) :
     global_SCH_recieveFullMsg ◁ᵥ global_SCH_recieveFullMsg @ function_ptr type_of_SCH_recieveFullMsg -∗
-    global_SML_switchTheSolenoid ◁ᵥ global_SML_switchTheSolenoid @ function_ptr type_of_SML_switchTheSolenoid -∗
-    typed_function (impl_SML_handleReceivedMsgs global_SCH_recieveFullMsg global_SML_switchTheSolenoid) type_of_SML_handleReceivedMsgs.
+    global_SML_trySwitch ◁ᵥ global_SML_trySwitch @ function_ptr type_of_SML_trySwitch -∗
+    typed_function (impl_SML_handleReceivedMsgs global_SCH_recieveFullMsg global_SML_trySwitch) type_of_SML_handleReceivedMsgs.
   Proof.
     Open Scope printing_sugar.
     start_function "SML_handleReceivedMsgs" ([[state msg] p]) => arg_ssp local_rxMsgSize.
@@ -24,11 +24,6 @@ Section proof_SML_handleReceivedMsgs.
     - repeat liRStep; liShow.
       all: print_typesystem_goal "SML_handleReceivedMsgs" "#0".
     Unshelve. all: li_unshelve_sidecond; sidecond_hook; prepare_sideconditions; normalize_and_simpl_goal; try solve_goal; unsolved_sidecond_hook.
-    + exists 8%nat. left. auto. intros [_ [_ HH1]]. rewrite HH1. auto.
-    + exists 8%nat. left. auto. intros [_ [_ HH1]]. rewrite HH1. auto.
-    + exists 0%nat. right. auto. 
-    + exists 0%nat. right. auto. 
-    + exists 0%nat. right. auto. 
     all: print_sidecondition_goal "SML_handleReceivedMsgs".
     Unshelve. all: try done; try apply: inhabitant; print_remaining_shelved_goal "SML_handleReceivedMsgs".
   Qed.
