src/proofs/solswitch/generated_proof_SML_trySwitch.v
@@ -1,0 +1,29 @@
+From refinedc.typing Require Import typing.
+From refinedc.project.learning.src.solswitch Require Import generated_code.
+From refinedc.project.learning.src.solswitch Require Import generated_spec.
+Set Default Proof Using "Type".
+
+(* Generated from [src/solswitch.c]. *)
+Section proof_SML_trySwitch.
+  Context `{!typeG Σ} `{!globalG Σ}.
+
+  (* Typing proof for [SML_trySwitch]. *)
+  Lemma type_SML_trySwitch (global_SML_switchTheSolenoid : loc) :
+    global_SML_switchTheSolenoid ◁ᵥ global_SML_switchTheSolenoid @ function_ptr type_of_SML_switchTheSolenoid -∗
+    typed_function (impl_SML_trySwitch global_SML_switchTheSolenoid) type_of_SML_trySwitch.
+  Proof.
+    Open Scope printing_sugar.
+    start_function "SML_trySwitch" ([[[state msg] len] p]) => arg_ssp arg_length.
+    prepare_parameters (state msg len p).
+    split_blocks ((
+      ∅
+    )%I : gmap label (iProp Σ)) ((
+      ∅
+    )%I : gmap label (iProp Σ)).
+    - repeat liRStep; liShow.
+      all: print_typesystem_goal "SML_trySwitch" "#0".
+    Unshelve. all: li_unshelve_sidecond; sidecond_hook; prepare_sideconditions; normalize_and_simpl_goal; try solve_goal; unsolved_sidecond_hook.
+    all: print_sidecondition_goal "SML_trySwitch".
+    Unshelve. all: try done; try apply: inhabitant; print_remaining_shelved_goal "SML_trySwitch".
+  Qed.
+End proof_SML_trySwitch.
